State2.thy
@@ -1,0 +1,107 @@
+theory State2 
+  imports Current
+begin
+
+datatype 'a idle = Idle "'a stack" nat
+
+fun idleToList :: "'a idle \<Rightarrow> 'a list" where
+  "idleToList (Idle stack _) = Stack.toList stack"
+
+datatype 'a common = 
+    Copy "'a current" "'a list" "'a list" nat
+  | Idle "'a idle"
+
+fun commonToList :: "'a common \<Rightarrow> 'a list" where
+  "commonToList (Idle idle) = idleToList idle"
+| "commonToList (Copy current _ _ _) = toList current"
+
+fun normalize :: "'a common \<Rightarrow> 'a common" where
+  "normalize (Copy current old new moved) = (
+      case current of Current extra added _ remained \<Rightarrow> 
+      if moved = remained
+      then Idle (idle.Idle (Stack extra new) (added + moved))
+      else Copy current old new moved
+  )"
+| "normalize state = state"
+
+fun tickCommon :: "'a common \<Rightarrow> 'a common" where
+  "tickCommon (Idle idle) = Idle idle"
+| "tickCommon (Copy current aux new moved) = (
+    case current of Current _ _ _ remained \<Rightarrow>
+      if moved < remained
+      then normalize (Copy current (tl aux) ((hd aux)#new) (moved + 1))
+      else normalize (Copy current aux new moved)
+  )"
+
+fun pushCommon :: "'a \<Rightarrow> 'a common \<Rightarrow> 'a common" where
+  "pushCommon x (Idle (idle.Idle stack stackSize)) = 
+      Idle (idle.Idle (push x stack) (Suc stackSize))"
+| "pushCommon x (Copy current aux new moved) = Copy (put x current) aux new moved"
+
+fun popCommon :: "'a common \<Rightarrow> 'a * 'a common" where
+  "popCommon (Idle (idle.Idle stack stackSize)) = 
+      (first stack, Idle (idle.Idle (pop stack) (stackSize - 1)))"
+| "popCommon (Copy current aux new moved) = 
+      (top current, Copy (bottom current) aux new moved)"
+
+datatype 'a stateB = 
+     Reverse "'a current" "'a stack" "'a list" nat
+   | Common "'a common"
+
+fun bToList :: "'a stateB \<Rightarrow> 'a list" where
+  "bToList (Common common) = commonToList common"
+| "bToList (Reverse current _ _ _) = toList current"
+
+fun tickB :: "'a stateB \<Rightarrow> 'a stateB" where
+  "tickB (Common state) = Common (tickCommon state)"
+| "tickB (Reverse current big auxB count) = 
+     Reverse current (pop big) ((first big)#auxB) (count - 1)"
+
+fun pushB :: "'a \<Rightarrow> 'a stateB \<Rightarrow> 'a stateB" where
+  "pushB x (Common state) = Common (pushCommon x state)"
+| "pushB x (Reverse current big auxB count) = Reverse (put x current) big auxB count"
+
+fun popB :: "'a stateB \<Rightarrow> 'a * 'a stateB" where
+  "popB (Common state) = (let (x, state) = popCommon state in (x, Common state))"
+| "popB (Reverse current big auxB count) = (top current, Reverse (bottom current) big auxB count)"
+
+datatype 'a stateS = 
+   Reverse1 "'a current" "'a stack" "'a list"
+ | Reverse2 "'a current" "'a list" "'a stack" "'a list" nat
+ | Common "'a common"
+
+fun sToList :: "'a stateS \<Rightarrow> 'a list" where
+  "sToList (Common common) = commonToList common"
+| "sToList (Reverse1 current _ _ ) = toList current"
+| "sToList (Reverse2 current _ _ _ _) = toList current"
+
+fun tickS :: "'a stateS \<Rightarrow> 'a stateS" where
+  "tickS (Common state) = Common (tickCommon state)"
+| "tickS (Reverse1 current small auxS) = (
+    if isEmpty small 
+    then Reverse1 current small auxS 
+    else Reverse1 current (pop small) ((first small)#auxS)
+  )"
+| "tickS (Reverse2 current auxS big newS count) = (
+    if isEmpty big
+    then Common (normalize (Copy current auxS newS count))
+    else Reverse2 current auxS (pop big) ((first big)#newS) (count + 1)
+  )"
+
+fun pushS :: "'a \<Rightarrow> 'a stateS \<Rightarrow> 'a stateS" where
+  "pushS x (Common state) = Common (pushCommon x state)"
+| "pushS x (Reverse1 current small auxS) = Reverse1 (put x current) small auxS"
+| "pushS x (Reverse2 current auxS big newS count) = Reverse2 (put x current) auxS big newS count"
+
+fun popS :: "'a stateS \<Rightarrow> 'a * 'a stateS" where
+  "popS (Common state) = (let (x, state) = popCommon state in (x, Common state))"
+| "popS (Reverse1 current small auxS) = (top current, Reverse1 (bottom current) small auxS)"
+| "popS (Reverse2 current auxS big newS count) = 
+    (top current, Reverse2 (bottom current) auxS big newS count)"
+
+fun ticks :: "'a stateB \<Rightarrow> 'a stateS \<Rightarrow> 'a stateB * 'a stateS" where
+  "ticks (Reverse currentB big auxB 0) (Reverse1 currentS _ auxS) =
+    (stateB.Common (normalize (Copy currentB auxB [] 0)), Reverse2 currentS auxS big [] 0)"
+| "ticks left right = (tickB left, tickS right)"
+
+end
